books/evm/base.lisp
@@ -4,6 +4,11 @@
   (and (natp n)
        (< n 256)))
 
+(defun evm-byte-arrayp (array)
+  (if (consp array)
+      (and (evm-bytep (car array)) (evm-byte-arrayp (cdr array)))
+      (equal array nil)))
+
 (defun fix-byte (n)
   (let ((n-fixed (nfix n)))
     (if (zp n-fixed) 0
@@ -21,16 +26,12 @@
 (defun w-from-bytes (byte-list)
   (if (consp byte-list)
       (if (cdr byte-list)
-          (+ (* (car byte-list) 256)
+          (+ (* (fix-byte (car byte-list)) 256)
              (w-from-bytes (cdr byte-list)))
-          (car byte-list))
+          (fix-byte (car byte-list)))
       0))
 
 (defun w-to-bytes (n byte-len)
   (if (zp byte-len) nil
       (append (w-to-bytes (floor n 256) (1- byte-len))
               (list (mod n 256)))))
-
-(defun evm-repeat (n x)
-  (if (zp n) nil
-      (cons x (evm-repeat (1- n) x))))
